[riscv] Adapt close_mmio_write to rely on a register instead of an immediate value.

case_study/RiscvPmp/BlockVer/Spec.v
@@ -594,8 +594,8 @@ Module RiscvPmpBlockVerifSpec <: Specification RiscvPmpBase RiscvPmpSignature Ri
   Import TermNotations.
 
   Definition lemma_close_mmio_write (immm : bv 12) (widthh : WordWidth): SepLemma (close_mmio_write immm widthh) :=
-    {| lemma_logic_variables := ["paddr" :: ty_xlenbits; "w" :: ty_xlenbits];
-       lemma_patterns        := [term_var "paddr"; term_var "w"];
+    {| lemma_logic_variables := ["paddr" :: ty_xlenbits; "r" :: ty_regno; "w" :: ty_word];
+       lemma_patterns        := [term_var "paddr"; term_var "r"];
        lemma_precondition    :=
         (term_val ty_xlenbits write_addr) = (term_var "paddr" +ᵇ term_sext (term_val (ty.bvec 12) immm)) ∨
         ((term_val ty_xlenbits write_addr_adv) = (term_var "paddr" +ᵇ term_sext (term_val (ty.bvec 12) immm)) ∗
