case_study/RiscvPmp/FemtoKernel.v
@@ -224,7 +224,7 @@ Module inv := invariants.
     Example femtokernel_handler_asm : list ASM :=
       [
         ITYPE (bv.of_N 42) zero t0 RISCV_ADDI
-      ; AnnotLemmaInvocation (close_mmio_write (bv.of_N mmio_write_addr) WORD) [nenv exp_val ty_xlenbits bv.zero; exp_val ty_xlenbits (bv.of_N 42)]%env (* TODO: notation to avoid lemma call copying LOAD instruction/internalize immediate as well?*)
+      ; AnnotLemmaInvocation (close_mmio_write (bv.of_N mmio_write_addr) WORD) [nenv exp_val ty_xlenbits bv.zero;  exp_val ty_regno t0]%env (* TODO: notation to avoid lemma call copying LOAD instruction/internalize immediate as well?*)
       ; STORE (bv.of_N mmio_write_addr) t0 zero WORD (* works because mmio_write_addr fits into 12 bits. *)
       ; MRET
       ].
@@ -260,7 +260,7 @@ Module inv := invariants.
        Jumps to femtokernel_handler_exit_asm at the end of the block.*)
     Example femtokernel_handler_write_asm (handler_exit_addr : N) : list AnnotInstr :=
       [ ADDI t0 zero (bv.of_N 42)
-      ; AnnotLemmaInvocation (close_mmio_write (bv.of_N mmio_write_adv) WORD) [nenv exp_val ty_xlenbits bv.zero; exp_val ty_xlenbits (bv.of_N 42)]%env
+      ; AnnotLemmaInvocation (close_mmio_write (bv.of_N mmio_write_adv) WORD) [nenv exp_val ty_xlenbits bv.zero; exp_val ty_regno t0]%env
       ; STORE (bv.of_N mmio_write_adv) t0 zero WORD (* works because mmio_write_adv fits into 12 bits. *)
       ; RISCV_JALR (bv.of_N handler_exit_addr) zero zero (* works because we the exit block addr fits into 12 bits *)
       ].
